Core/Automata2.v
@@ -64,6 +64,9 @@ Record ctransition :=
       tfun : trans_fun_type;
   }.
 
+Definition idle_fun : trans_fun_type := fun _ _ s _ _ => (s, None).
+Definition idle := CTrans 0 idle_fun.
+
 End Transitions.
 
 Record Protocol (S : Type) :=
@@ -79,6 +82,9 @@ Record Protocol (S : Type) :=
       (* All transitions have unique tags *)
       _ : uniq (map (@ttag _) transitions)
     }.
+
+Definition tags {S : Type} (p : Protocol S) :=
+  map (@ttag _) (transitions p).
 
 End Protocol.
 
@@ -96,20 +102,107 @@ Fixpoint wf_sched (sch : schedule) :=
        all [pred s' | bnum <= block_num s'.1] sch' && wf_sched sch'
   else true.
 
-(* TODO: Define traces of the protocol wrt. a schedule as sequences of *)
-(* triplets *)
+Record step :=
+  Step {
+      pre  : cstate S;
+      post : cstate S;
+      out  : option message                                            
+  }.
 
-(* TODO: Define safety properties as something that holds over every *)
-(* triplet; provide and induction principle for this *)
+Definition trace := seq step.
 
-(* TODO: define semantics for blockchain-schedules: 
+Definition apply_prot id bal s m bc : (S * option message) :=
+  let n  := seq.find (fun t => ttag t == method m) (transitions p) in
+  let tr := nth (idle S) (transitions p) n in
+  let f  := tfun tr in
+  f id bal s m bc.
 
-- Each components in the schedule has a timestamp, and an incoming message;
-- In good schedules, schedules timestamps are (non-strictly) growing;
-- Goodness also ensures that all messages are well-formed wrt. the tag;
-- Contract functions are total, so we handle all incoming messages;
+Definition step_prot pre bc m : step :=
+  let: CState id bal s := pre in
+  let: (s', out) := apply_prot id bal s m bc in
+  let: bal' := if out is Some m' then (bal + val m) - val m' else bal in
+  let: post := CState id bal' s' in
+  Step pre post out.
+
+(* Map a schedule into a trace *)
+Fixpoint execute (pre : cstate S) (sc: schedule) : trace :=
+  if sc is (bc, m) :: sc'
+  then let stp := step_prot pre bc m in
+       stp :: execute (post stp) sc' 
+  else [::].
+
+Definition state0 := CState (acc p) (init_bal p) (init_state p).
+
+(* Execute from the initial contract state,
+   if schedule is empty, repeat the initial state *)
+Definition execute0 sc :=
+  if sc is _ :: _
+  then execute state0 sc
+  else [:: Step state0 state0 None].
+
+(****************************************************************)
+(* Safety property:
+
+For any state s in _any_ trace, starting from the initial one, 
+the unary property I holds (i.e., I s).
+
 *)
+(****************************************************************)
+Definition safe (I : cstate S -> Prop) : Prop :=
+  forall sc pre post out,
+    Step pre post out \In execute0 sc -> I pre /\ I post.
 
+Lemma bad_tag_step bc m s :
+  method m \notin (tags p) -> post (step_prot s bc m) = s.
+Proof.
+move=>M; rewrite /step_prot; case: s=>id bal s.
+rewrite [apply_prot _ _ _ _ _]surjective_pairing/=.
+rewrite /apply_prot.
+suff X : seq.find (fun t : ctransition S => ttag t == method m) (transitions p) =
+         size (transitions p).
+by rewrite !X !nth_default ?leqnn//. 
+move: (find_size (fun t : ctransition S => ttag t == method m) (transitions p)).
+rewrite leq_eqVlt; case/orP; first by move/eqP.
+rewrite -has_find=>G. suff X: False by [].
+rewrite /tags in M; clear s bal id bc.
+elim: (transitions p) G M=>//t ts Hi/=.
+case/orP; last by move/Hi=>{Hi} Hi H; apply: Hi; rewrite inE in H; case/norP: H. 
+by move/eqP=>->; rewrite inE eqxx.
+Qed.
+
+(* A strong induction principle for proving safety *)
+Lemma safe_ind (I : cstate S -> Prop) :
+  I state0 ->
+  (forall pre bc m, (method m \in tags p) -> I pre -> I (post (step_prot pre bc m))) ->
+  safe I.
+Proof.
+move=>H1 H2; case=>[|[bc m] sc] pre pst out; first by case=>[][->->].
+case/In_cons=>[E|];[| rewrite -/execute].
+- have Z: pst = post (step_prot state0 bc m) by rewrite -E.
+  subst pst; split. 
+  + suff Z: pre = state0 by subst pre.
+    move: E; rewrite /step_prot/=.
+    by rewrite [apply_prot _ _ _ _ _]surjective_pairing; case.  
+  case M: (method m \in tags p); first by apply: H2.
+  by rewrite bad_tag_step// M.  
+have Hp: I (post (step_prot state0 bc m)).
+- case M: (method m \in tags p); first by apply: H2.
+  by rewrite bad_tag_step// M.   
+move: (post (step_prot state0 bc m)) Hp=>s Hi G; clear H1 bc m.
+elim: sc s Hi G=>//[[bc m] sc] Hi s Is.
+case/In_cons=>[E|];[|rewrite -/execute]; last first.
+- move/Hi=>H; apply: H.
+  case M: (method m \in tags p); first by apply: H2.
+  by rewrite bad_tag_step// M.   
+suff Z: s = pre /\ pst = post (step_prot pre bc m).
+- case: Z=>??; subst pre pst; split=>//.
+  case M: (method m \in tags p); first by apply: H2.
+  by rewrite bad_tag_step// M.   
+move: E; rewrite /step_prot/=; clear Is.
+case: s=>id bal s; rewrite [apply_prot _ _ _ _ _]surjective_pairing.
+by case=>->; rewrite {4}[apply_prot id bal s m bc]surjective_pairing. 
+Qed.
+ 
 
 End Semantics.
 
